%2multibyte Version: 5.50.0.2953 CodePage: 65001

\documentclass{article}
%%%%%%%%%%%%%%%%%%%%%%%%%%%%%%%%%%%%%%%%%%%%%%%%%%%%%%%%%%%%%%%%%%%%%%%%%%%%%%%%%%%%%%%%%%%%%%%%%%%%%%%%%%%%%%%%%%%%%%%%%%%%%%%%%%%%%%%%%%%%%%%%%%%%%%%%%%%%%%%%%%%%%%%%%%%%%%%%%%%%%%%%%%%%%%%%%%%%%%%%%%%%%%%%%%%%%%%%%%%%%%%%%%%%%%%%%%%%%%%%%%%%%%%%%%%%
%TCIDATA{OutputFilter=LATEX.DLL}
%TCIDATA{Version=5.50.0.2953}
%TCIDATA{Codepage=65001}
%TCIDATA{<META NAME="SaveForMode" CONTENT="1">}
%TCIDATA{BibliographyScheme=Manual}
%TCIDATA{Created=Sunday, July 21, 2013 13:10:11}
%TCIDATA{LastRevised=Tuesday, July 23, 2013 19:30:56}
%TCIDATA{<META NAME="GraphicsSave" CONTENT="32">}
%TCIDATA{<META NAME="DocumentShell" CONTENT="Scientific Notebook\Blank Document">}
%TCIDATA{CSTFile=Math with theorems suppressed.cst}
%TCIDATA{PageSetup=72,72,72,72,0}
%TCIDATA{AllPages=
%F=36,\PARA{038<p type="texpara" tag="Body Text" >\hfill \thepage}
%}


\newtheorem{theorem}{Theorem}
\newtheorem{acknowledgement}[theorem]{Acknowledgement}
\newtheorem{algorithm}[theorem]{Algorithm}
\newtheorem{axiom}[theorem]{Axiom}
\newtheorem{case}[theorem]{Case}
\newtheorem{claim}[theorem]{Claim}
\newtheorem{conclusion}[theorem]{Conclusion}
\newtheorem{condition}[theorem]{Condition}
\newtheorem{conjecture}[theorem]{Conjecture}
\newtheorem{corollary}[theorem]{Corollary}
\newtheorem{criterion}[theorem]{Criterion}
\newtheorem{definition}[theorem]{Definition}
\newtheorem{example}[theorem]{Example}
\newtheorem{exercise}[theorem]{Exercise}
\newtheorem{lemma}[theorem]{Lemma}
\newtheorem{notation}[theorem]{Notation}
\newtheorem{problem}[theorem]{Problem}
\newtheorem{proposition}[theorem]{Proposition}
\newtheorem{remark}[theorem]{Remark}
\newtheorem{solution}[theorem]{Solution}
\newtheorem{summary}[theorem]{Summary}
\newenvironment{proof}[1][Proof]{\noindent\textbf{#1.} }{\ \rule{0.5em}{0.5em}}
\input{tcilatex}
\begin{document}


The Equilibrium conditions of the model

\begin{equation}
y_{t}=c_{t}+g_{t}
\end{equation}

\begin{equation}
y_{t}=A_{t}n_{t}
\end{equation}

\begin{equation}
A_{t}-a=\rho _{A}\left( A_{t-1}-a\right) +\sigma _{A}\varepsilon _{A,t}
\end{equation}

\begin{equation}
\tau _{t}y_{t}+b_{t}q_{t}=\left( 1-\Delta \left( v_{t}\right) \right)
b_{t-1}+g_{t}+z_{t}
\end{equation}

\begin{equation}
s_{t}=\frac{b_{t}}{y_{t}}
\end{equation}%
\begin{equation}
\tau _{t}=\left( 1-\rho _{\tau }\right) \tau +\rho _{\tau }\tau
_{t-1}+\sigma _{\tau }\varepsilon _{\tau ,t}+\gamma _{\tau }\left(
b_{t}^{d}-b\right)
\end{equation}%
\begin{equation}
b_{t}^{d}=\left( 1-\Delta \left( v_{t}\right) \right) b_{t-1}
\end{equation}

\begin{equation}
g_{t}-g=\rho _{g}\left( g_{t-1}-g\right) +\sigma _{g}\varepsilon _{g,t}
\end{equation}

\begin{equation}
z_{t}-z=\rho _{z}\left( z_{t-1}-z\right) +\sigma _{z}\varepsilon _{z,t}
\end{equation}

\begin{equation}
\phi \frac{c_{t}-hc_{t-1}}{1-n_{t}}=A_{t}\left( 1-\tau _{t}\right)
\end{equation}

\begin{equation}
q_{t}=\beta \left( 1-\Delta \left( v_{t}\right) \right) \left( \frac{%
c_{t}-hc_{t-1}}{c_{t+1}-hc_{t}}\right) 
\end{equation}

Endogenous list: $y_{t},c_{t},g_{t},A_{t},n_{t},\tau
_{t},b_{t},q_{t},z_{t},s_{t},b_{t}^{d}$

The steady state

$a=1$

$\frac{b}{y}=1.095$

$\frac{g}{y}=0.181$

$\tau =1/3$

$n_{t}=0.25$

\[
\Delta \left( v_{t}\right) =0
\]

\begin{equation}
A_{t}=a
\end{equation}%
\begin{equation}
\tau _{t}=\tau 
\end{equation}

\begin{equation}
n_{t}=0.25
\end{equation}

\begin{equation}
y_{t}=A_{t}n_{t}
\end{equation}

\begin{equation}
g_{t}=g=\left( \frac{g}{y}\right) y_{t}
\end{equation}

\begin{equation}
c_{t}=y_{t}-g_{t}
\end{equation}

\begin{equation}
b_{t}=\left( \frac{b_{t}}{y_{t}}\right) y_{t}
\end{equation}

\begin{equation}
z_{t}=z=\left[ \tau _{t}-\frac{b_{t}}{y_{t}}\left( 1-\beta \right) \left(
1-\Delta \left( v_{t}\right) \right) -\frac{g_{t}}{y_{t}}\right] y_{t}
\end{equation}

\begin{equation}
q_{t}=\beta \left( 1-\Delta \left( v_{t}\right) \right) 
\end{equation}

\begin{equation}
s_{t}=\frac{b_{t}}{y_{t}}
\end{equation}%
\begin{equation}
b_{t}^{d}=\left( 1-\Delta \left( v_{t}\right) \right) b_{t}
\end{equation}

\end{document}
